specs/Spec.Stream.fsti
@@ -11,6 +11,7 @@ module U32 = FStar.UInt32
 module U8 = FStar.UInt8
 
 open Lib.Seq
+open Yazi.Stream.Types
 
 type stream_state = s:Seq.seq U32.t{Seq.length s == 5}
 
@@ -19,6 +20,12 @@ unfold let total_in (s: stream_state) = U32.v s.[1]
 unfold let avail_out (s: stream_state) = U32.v s.[2]
 unfold let total_out (s: stream_state) = U32.v s.[3]
 unfold let adler (s: stream_state) = s.[4]
+
+unfold let avail_in_unchange (s0 s1: stream_state) = U32.v s0.[0] == U32.v s1.[0]
+unfold let total_in_unchange (s0 s1: stream_state) = U32.v s0.[1] == U32.v s1.[1]
+unfold let avail_out_unchange (s0 s1: stream_state) = U32.v s0.[2] == U32.v s1.[2]
+unfold let total_out_unchange (s0 s1: stream_state) = U32.v s0.[3] == U32.v s1.[3]
+unfold let adler_unchange (s0 s1: stream_state) = U32.v s0.[4] == U32.v s1.[4]
 
 unfold let next_in_valid
   (h: HS.mem)
@@ -44,7 +51,7 @@ unfold let next_out_valid
 
 unfold let adler_valid
   (h: HS.mem)
-  (s: B.lbuffer U32.t 5)
+  (s: stream_state_t)
   (wrap: I32.t)
   (uncompressed: Seq.seq U8.t) =
   let s' = B.as_seq h s in
@@ -56,7 +63,7 @@ unfold let adler_valid
 
 let stream_valid
   (h: HS.mem)
-  (s: B.lbuffer U32.t 5)
+  (s: stream_state_t)
   (next_in: B.pointer (B.buffer U8.t))
   (next_out: B.pointer (B.buffer U8.t))
   (wrap: I32.t)
@@ -73,3 +80,53 @@ let stream_valid
 
   next_in_valid h s next_in /\ next_out_valid h s next_out /\
   adler_valid h s wrap uncompressed
+
+private unfold let read_buf_size(h: HS.mem) (s: stream_state_t) (size: U32.t) =
+  let s' = B.as_seq h s in
+  if U32.v size > avail_in s' then avail_in s' else U32.v size
+
+let read_buf_pre
+  (h: HS.mem)
+  (s: stream_state_t)
+  (uncompressed: Seq.seq U8.t)
+  (next_in: B.pointer (B.buffer U8.t))
+  (buf: B.buffer U8.t)
+  (size: U32.t)
+  (wrap: I32.t) =
+  let len = read_buf_size h s size in
+  len > 0 /\
+  B.live h s /\ ~(B.g_is_null s) /\
+  B.live h buf /\ ~(B.g_is_null buf) /\
+  HS.disjoint (B.frameOf s) (B.frameOf buf) /\
+  B.length buf == U32.v size /\
+  next_in_valid h s next_in /\
+  adler_valid h s wrap uncompressed
+
+let read_buf_post
+  (h0: HS.mem)
+  (res: (U32.t & Ghost.erased (B.buffer U8.t)))
+  (h1: HS.mem)
+  (s: stream_state_t)
+  (uncompressed: Seq.seq U8.t)
+  (next_in: B.pointer (B.buffer U8.t))
+  (buf: B.buffer U8.t)
+  (size: U32.t)
+  (wrap: I32.t) =
+  let (len', read) = res in
+  let next_in0 = B.get h0 next_in 0 in
+  let next_in1 = B.get h1 next_in 0 in
+  let s0 = B.as_seq h0 s in
+  let s1 = B.as_seq h1 s in
+  let len = read_buf_size h0 s size in
+  len == U32.v len' /\
+  B.modifies (
+    B.loc_buffer s `B.loc_union`
+    B.loc_buffer next_in `B.loc_union`
+    B.loc_buffer buf) h0 h1 /\
+  U32.v len' <= B.length next_in0 /\
+  Seq.equal (B.as_seq h1 read) (B.as_seq h0 (B.gsub next_in0 0ul len')) /\
+  avail_in s0 - len == avail_in s1 /\
+  next_in_valid h1 s next_in /\
+  adler_valid h1 s wrap (Seq.append uncompressed (B.as_seq h1 read)) /\
+  avail_out_unchange s0 s1 /\
+  total_out_unchange s0 s1
